Add some helpers for cleaner tests, WIP transitivity typing

translation/TestEquality.v
@@ -1,5 +1,6 @@
 Require Import Helpers.
 Require Import Library.
+Require Import TestHelpers.
 Require Import GMu.TestEquality.
 Require Import Translation.
 
@@ -58,21 +59,68 @@ Eval cbv in p_coerce_typ.
      : typ
  *)
 
-(* TODO: issue DeBruijn is not shared in L2GMu but is shared in pDOT! *)
+
+Definition make_fun_apply (f : trm) (arg : trm) : trm :=
+  match f with
+  | trm_path pf =>
+    match arg with
+    | trm_path pa =>
+      trm_app pf pa
+    | _ =>
+      trm_let arg (trm_app (shift1_p pf) this)
+    end
+  | _ =>
+    trm_let
+      f
+      (trm_let (shift1_trm arg)
+               (trm_app super this)
+      )
+  end.
+
+Notation "f $ a" := (make_fun_apply f a) (at level 42).
+
+Definition TLgen (T : typ) : trm :=
+  let inner := shift1_typ T in
+  let_trm (ν({GenT == inner}) {( {GenT ⦂= inner} )}).
+
+Section TestApp.
+  Definition a := trm_path this.
+  Definition b := trm_path super.
+  Definition c := trm_path ssuper.
+
+  Axiom A B C : var.
+
+  Definition sub (t : trm) : trm :=
+    open_rec_trm_p 2 (pvar C) (open_rec_trm_p 1 (pvar B) (open_trm_p (pvar A) t)).
+
+  Goal sub b = tvar B.
+    cbv. crush.
+  Qed.
+  Goal sub a = tvar A.
+    cbv. crush.
+  Qed.
+  Goal sub c = tvar C.
+    cbv. crush.
+  Qed.
+
+  Definition t :=
+    a $ b $ c.
+
+  Goal sub t = tvar A $ tvar B $ tvar C.
+    cbv.
+    crush.
+  Qed.
+
+  Eval cbv in tvar A $ tvar B $ tvar C.
+End TestApp.
+
 Definition p_coerce_trm : trm :=
   λ ({GenT >: ⊥ <: ⊤}) λ ({GenT >: ⊥ <: ⊤})
     λ (((pvar env ↓ GN Eq) ∧ {Ai 1 == this ↓ GenT}) ∧ {Ai 2 == super ↓ GenT})
     λ (ssuper ↓ GenT)
     trm_let
-    (let_trm (ν({GenT == sssuper ↓ GenT}) {( {GenT ⦂= sssuper ↓ GenT} )} ))
-    (trm_let
-       (λ (pvar env ↓ GC Eq 0 ∧ {{ssuper}}) trm_path ssuper)
-       (trm_let
-          (trm_app (sssuper • pmatch) super)
-          (let_trm (trm_app this super))
-       )
-    )
-    .
+    (TLgen (ref 2 ↓ GenT))
+    (trm_path ssuper • pmatch $ trm_path this $ (λ (pvar env ↓ GC Eq 0 ∧ {{ssuper}}) trm_path ssuper)).
 
 Ltac cleanup :=
   repeat
@@ -127,98 +175,14 @@ Lemma p_coerce_types :
       rewrite <- HR at 2.
       apply ty_rec_elim. crush.
   - cleanup.
-    apply_fresh ty_let as c0case; crush.
-    + instantiate (1:= ∀ (pvar env ↓ GC Eq 0 ∧ {{pvar eq}} ) (pvar TL ↓ GenT) ).
-      repeat rewrite <- Heqenv.
-      apply_fresh ty_all_intro as eq_ev; crush.
-      apply ty_sub with (pvar A ↓ GenT).
-      * apply ty_var. crush.
-      * apply subtyp_trans with (pvar B ↓ GenT).
-        2: {
-          eapply subtyp_sel2.
-          crush.
-        }
-        apply subtyp_trans with (pvar eq_ev ↓ Bi 1).
-        -- apply subtyp_trans with (pvar eq ↓ Ai 2).
-           ++ eapply subtyp_sel2.
-              var_subtyp; crush.
-           ++ apply subtyp_trans with (pvar eq_ev ↓ Ai 2).
-              ** eapply subtyp_sngl_qp with (p := pvar eq_ev) (q := pvar eq);
-                   try solve [var_subtyp; crush].
-                 assert (HR: pvar eq_ev = (pvar eq_ev) •• []) by crush.
-                 rewrite HR at 2.
-                 assert (HR2: pvar eq = (pvar eq) •• []) by crush.
-                 rewrite HR2 at 2.
-                 apply rpath.
-              ** eapply subtyp_sel1.
-                 apply ty_sub with (((((pvar env ↓ GN Eq) ∧ {Bi 1 >: ⊥ <: ⊤}) ∧ {Ai 1 == pvar eq_ev ↓ Bi 1}) ∧ {Ai 2 == pvar eq_ev ↓ Bi 1}) ∧ {data ⦂ pvar lib ↓ Unit}).
-                 ---
-                   assert (HR:
-                             ((((pvar env ↓ GN Eq) ∧ {Bi 1 >: ⊥ <: ⊤}) ∧ {Ai 1 == pvar eq_ev ↓ Bi 1})
-                              ∧ {Ai 2 == pvar eq_ev ↓ Bi 1}) ∧ {data ⦂ pvar lib ↓ Unit}
-                                      =
-                                      open_typ_p (pvar eq_ev) (((((pvar env ↓ GN Eq) ∧ {Bi 1 >: ⊥ <: ⊤}) ∧ {Ai 1 == this ↓ Bi 1}) ∧ {Ai 2 == this ↓ Bi 1}) ∧ {data ⦂ pvar lib ↓ Unit})) by crush.
-                   rewrite HR.
-                   apply ty_rec_elim.
-                   apply ty_sub with (pvar env ↓ GC Eq 0).
-                   +++ var_subtyp; crush.
-                   +++ eapply subtyp_sel1.
-                       match goal with
-                       | [ |- context [ env ~ μ ?T ] ] =>
-                         apply ty_sub with (open_typ_p (pvar env) T)
-                       end.
-                       *** apply ty_rec_elim. apply ty_var.
-                           solve_bind.
-                       *** crush.
-                           eapply subtyp_trans; try apply subtyp_and11.
-                           apply subtyp_and12.
-                 --- eapply subtyp_trans; try apply subtyp_and11.
-                     apply subtyp_and12.
-        -- apply subtyp_trans with (pvar eq ↓ Ai 1).
-           ++ apply subtyp_trans with (pvar eq_ev ↓ Ai 1).
-              ** eapply subtyp_sel2.
-                 apply ty_sub with (((((pvar env ↓ GN Eq) ∧ {Bi 1 >: ⊥ <: ⊤}) ∧ {Ai 1 == pvar eq_ev ↓ Bi 1}) ∧ {Ai 2 == pvar eq_ev ↓ Bi 1}) ∧ {data ⦂ pvar lib ↓ Unit}).
-                 ---
-                   assert (HR:
-                             ((((pvar env ↓ GN Eq) ∧ {Bi 1 >: ⊥ <: ⊤}) ∧ {Ai 1 == pvar eq_ev ↓ Bi 1})
-                              ∧ {Ai 2 == pvar eq_ev ↓ Bi 1}) ∧ {data ⦂ pvar lib ↓ Unit}
-                                      =
-                                      open_typ_p (pvar eq_ev) (((((pvar env ↓ GN Eq) ∧ {Bi 1 >: ⊥ <: ⊤}) ∧ {Ai 1 == this ↓ Bi 1}) ∧ {Ai 2 == this ↓ Bi 1}) ∧ {data ⦂ pvar lib ↓ Unit})) by crush.
-                   rewrite HR.
-                   apply ty_rec_elim.
-                   apply ty_sub with (pvar env ↓ GC Eq 0).
-                   +++ var_subtyp; crush.
-                   +++ eapply subtyp_sel1.
-                       match goal with
-                       | [ |- context [ env ~ μ ?T ] ] =>
-                         apply ty_sub with (open_typ_p (pvar env) T)
-                       end.
-                       *** apply ty_rec_elim. apply ty_var.
-                           solve_bind.
-                       *** crush.
-                           eapply subtyp_trans; try apply subtyp_and11.
-                           apply subtyp_and12.
-                 --- eapply subtyp_trans; try apply subtyp_and11.
-                     eapply subtyp_trans; try apply subtyp_and11.
-                     apply subtyp_and12.
-              ** eapply subtyp_sngl_pq with (p := pvar eq_ev) (q := pvar eq);
-                   try solve [var_subtyp; crush].
-                 assert (HR: pvar eq_ev = (pvar eq_ev) •• []) by crush.
-                 rewrite HR at 2.
-                 assert (HR2: pvar eq = (pvar eq) •• []) by crush.
-                 rewrite HR2 at 2.
-                 apply rpath.
-           ++ eapply subtyp_sel1.
-              var_subtyp; crush.
-              eapply subtyp_trans; try apply subtyp_and11.
-              apply subtyp_and12.
-    + apply_fresh ty_let as app_tmp1; crush.
-      * instantiate (1:= open_typ_p (pvar TL) (∀ ( ∀ (pvar env ↓ GC Eq 0 ∧ {{pvar eq}} ) (super ↓ GenT) ) (super ↓ GenT))).
-        eapply ty_all_elim.
-        2: {
-          apply ty_var. crush.
-        }
-        assert (HR: p_sel (avar_f eq) [pmatch] = (pvar eq) • pmatch) by crush.
+    apply_fresh ty_let as app_tmp1; crush.
+    + instantiate (1:= open_typ_p (pvar TL) (∀ ( ∀ (pvar env ↓ GC Eq 0 ∧ {{pvar eq}} ) (super ↓ GenT) ) (super ↓ GenT))).
+
+      eapply ty_all_elim.
+      2: {
+        apply ty_var. crush.
+      }
+      assert (HR: p_sel (avar_f eq) [pmatch] = (pvar eq) • pmatch) by crush.
         rewrite HR.
 
         match goal with
@@ -247,16 +211,277 @@ Lemma p_coerce_types :
                     eapply subtyp_trans; try apply subtyp_and11.
           ++ crush.
         -- apply_fresh subtyp_all as TLL; crush.
-      * apply_fresh ty_let as res_tmp.
-        -- crush.
-           instantiate (1 := open_typ_p (pvar c0case) (pvar TL ↓ GenT)).
-           eapply ty_all_elim; crush.
-        -- crush.
-           apply ty_sub with (pvar TL ↓ GenT); crush.
-           eapply subtyp_sel1.
-           crush.
+    + apply_fresh ty_let as c0case; crush.
+      1: {
+        instantiate (1:= ∀ (pvar env ↓ GC Eq 0 ∧ {{pvar eq}} ) (pvar TL ↓ GenT) ).
+        repeat rewrite <- Heqenv.
+        apply_fresh ty_all_intro as eq_ev; crush.
+        apply ty_sub with (pvar A ↓ GenT).
+        * apply ty_var. crush.
+        * apply subtyp_trans with (pvar B ↓ GenT).
+          2: {
+            eapply subtyp_sel2.
+            crush.
+          }
+          apply subtyp_trans with (pvar eq_ev ↓ Bi 1).
+          -- apply subtyp_trans with (pvar eq ↓ Ai 2).
+             ++ eapply subtyp_sel2.
+                var_subtyp; crush.
+                apply ty_var. solve_bind.
+             ++ apply subtyp_trans with (pvar eq_ev ↓ Ai 2).
+                ** eapply subtyp_sngl_qp with (p := pvar eq_ev) (q := pvar eq);
+                     try solve [var_subtyp; crush; apply ty_var; solve_bind].
+                   assert (HR: pvar eq_ev = (pvar eq_ev) •• []) by crush.
+                   rewrite HR at 2.
+                   assert (HR2: pvar eq = (pvar eq) •• []) by crush.
+                   rewrite HR2 at 2.
+                   apply rpath.
+                ** eapply subtyp_sel1.
+                   apply ty_sub with (((((pvar env ↓ GN Eq) ∧ {Bi 1 >: ⊥ <: ⊤}) ∧ {Ai 1 == pvar eq_ev ↓ Bi 1}) ∧ {Ai 2 == pvar eq_ev ↓ Bi 1}) ∧ {data ⦂ pvar lib ↓ Unit}).
+                   ---
+                     assert (HR:
+                               ((((pvar env ↓ GN Eq) ∧ {Bi 1 >: ⊥ <: ⊤}) ∧ {Ai 1 == pvar eq_ev ↓ Bi 1})
+                                ∧ {Ai 2 == pvar eq_ev ↓ Bi 1}) ∧ {data ⦂ pvar lib ↓ Unit}
+                                                                 =
+                                                                 open_typ_p (pvar eq_ev) (((((pvar env ↓ GN Eq) ∧ {Bi 1 >: ⊥ <: ⊤}) ∧ {Ai 1 == this ↓ Bi 1}) ∧ {Ai 2 == this ↓ Bi 1}) ∧ {data ⦂ pvar lib ↓ Unit})) by crush.
+                     rewrite HR.
+                     apply ty_rec_elim.
+                     apply ty_sub with (pvar env ↓ GC Eq 0).
+                     +++ var_subtyp; crush.
+                     +++ eapply subtyp_sel1.
+                         match goal with
+                         | [ |- context [ env ~ μ ?T ] ] =>
+                           apply ty_sub with (open_typ_p (pvar env) T)
+                         end.
+                         *** apply ty_rec_elim. apply ty_var.
+                             solve_bind.
+                         *** crush.
+                             eapply subtyp_trans; try apply subtyp_and11.
+                             apply subtyp_and12.
+                   --- eapply subtyp_trans; try apply subtyp_and11.
+                       apply subtyp_and12.
+          -- apply subtyp_trans with (pvar eq ↓ Ai 1).
+             ++ apply subtyp_trans with (pvar eq_ev ↓ Ai 1).
+                ** eapply subtyp_sel2.
+                   apply ty_sub with (((((pvar env ↓ GN Eq) ∧ {Bi 1 >: ⊥ <: ⊤}) ∧ {Ai 1 == pvar eq_ev ↓ Bi 1}) ∧ {Ai 2 == pvar eq_ev ↓ Bi 1}) ∧ {data ⦂ pvar lib ↓ Unit}).
+                   ---
+                     assert (HR:
+                               ((((pvar env ↓ GN Eq) ∧ {Bi 1 >: ⊥ <: ⊤}) ∧ {Ai 1 == pvar eq_ev ↓ Bi 1})
+                                ∧ {Ai 2 == pvar eq_ev ↓ Bi 1}) ∧ {data ⦂ pvar lib ↓ Unit}
+                                                                 =
+                                                                 open_typ_p (pvar eq_ev) (((((pvar env ↓ GN Eq) ∧ {Bi 1 >: ⊥ <: ⊤}) ∧ {Ai 1 == this ↓ Bi 1}) ∧ {Ai 2 == this ↓ Bi 1}) ∧ {data ⦂ pvar lib ↓ Unit})) by crush.
+                     rewrite HR.
+                     apply ty_rec_elim.
+                     apply ty_sub with (pvar env ↓ GC Eq 0).
+                     +++ var_subtyp; crush.
+                     +++ eapply subtyp_sel1.
+                         match goal with
+                         | [ |- context [ env ~ μ ?T ] ] =>
+                           apply ty_sub with (open_typ_p (pvar env) T)
+                         end.
+                         *** apply ty_rec_elim. apply ty_var.
+                             solve_bind.
+                         *** crush.
+                             eapply subtyp_trans; try apply subtyp_and11.
+                             apply subtyp_and12.
+                   --- eapply subtyp_trans; try apply subtyp_and11.
+                       eapply subtyp_trans; try apply subtyp_and11.
+                       apply subtyp_and12.
+                ** eapply subtyp_sngl_pq with (p := pvar eq_ev) (q := pvar eq);
+                     try solve [var_subtyp; crush; apply ty_var; solve_bind].
+                   assert (HR: pvar eq_ev = (pvar eq_ev) •• []) by crush.
+                   rewrite HR at 2.
+                   assert (HR2: pvar eq = (pvar eq) •• []) by crush.
+                   rewrite HR2 at 2.
+                   apply rpath.
+             ++ eapply subtyp_sel1.
+                var_subtyp; crush; try (apply ty_var; solve_bind).
+                eapply subtyp_trans; try apply subtyp_and11.
+                apply subtyp_and12.
+      }
+
+crush.
+      apply ty_sub with (pvar TL ↓ GenT); crush.
+      * assert (HR: open_typ_p (pvar c0case) (pvar TL ↓ GenT) = pvar TL ↓ GenT) by crush.
+        rewrite <- HR.
+        eapply ty_all_elim; crush.
+      * crush.
+        eapply subtyp_sel1.
+        crush.
 Qed.
 
-Definition p_transitivity_typ := translateTyp0 transitivity_typ.
+Definition p_transitivity_typ : typ := translateTyp0 transitivity_typ.
 
 Eval cbv in p_transitivity_typ.
+(*
+     = ∀ ({GenT >: ⊥ <: ⊤}) (∀ ({GenT >: ⊥ <: ⊤}) (∀ ({GenT >: ⊥ <: ⊤})
+        (∀ (((pvar env ↓ GN Eq) ∧ {Ai 1 == super ↓ GenT}) ∧ {Ai 2 == ssuper ↓ GenT})
+         (∀ (((pvar env ↓ GN Eq) ∧ {Ai 1 == super ↓ GenT}) ∧ {Ai 2 == ssuper ↓ GenT})
+           (((pvar env ↓ GN Eq) ∧ {Ai 1 == ssuper ↓ GenT}) ∧ {Ai 2 == ssssuper ↓ GenT})))))
+     : Target.typ
+ *)
+
+Coercion trm_path : path >-> trm.
+
+Definition p_transitivity_trm : trm :=
+  λ (*A*) ({GenT >: ⊥ <: ⊤}) λ (*B*) ({GenT >: ⊥ <: ⊤}) λ (*C*) ({GenT >: ⊥ <: ⊤})
+    λ (*eq1*) (((pvar env ↓ GN Eq) ∧ {Ai 1 == (* B *) ref 1 ↓ GenT}) ∧ {Ai 2 == (* A *) ref 2 ↓ GenT})
+    λ (*eq2*) (((pvar env ↓ GN Eq) ∧ {Ai 1 == (* C *) ref 1 ↓ GenT}) ∧ {Ai 2 == (* B *) ref 2 ↓ GenT})
+    trm_let
+    (* TL = *)
+    (TLgen (((pvar env ↓ GN Eq) ∧ {Ai 1 == (* C *) ref 2 ↓ GenT}) ∧ {Ai 2 == (* A *) ref 4 ↓ GenT}))
+    (let_trm (
+      (ref 2) • pmatch $ ref 0 $
+              (λ (*eq1_ev *) (pvar env ↓ GC Eq 0 ∧ {{ ref 2 }})
+                 (ref 2) • pmatch $ ref 1 $
+                 (λ (*eq2_ev *) (pvar env ↓ GC Eq 0 ∧ {{ ref 2 }})
+                    (let_trm
+                       ((pvar env) • refl $ (ν({Bi 1 == ref 6 ↓ GenT}) {( {Bi 1 ⦂= ref 6 ↓ GenT} )} ))
+                    )
+                 )
+              )
+    ))
+.
+
+Lemma p_transitivity_types :
+  empty & lib ~ libType
+  & env ~ (open_typ_p (pvar lib) env_typ)
+        ⊢
+        p_transitivity_trm : p_transitivity_typ.
+  remember lib as lib.
+  remember env as env.
+  intros.
+  cbv.
+  crush.
+  apply_fresh ty_all_intro as A; crush.
+  apply_fresh ty_all_intro as B; crush.
+  cleanup.
+  apply_fresh ty_all_intro as C; crush.
+  apply_fresh ty_all_intro as eq1; crush.
+  apply_fresh ty_all_intro as eq2; crush.
+  apply_fresh ty_let as TL; crush.
+  1: {
+    instantiate (1:= {GenT == (pvar env ↓ GN Eq) ∧ {Ai 1 == pvar C ↓ GenT} ∧ {Ai 2 == (pvar A) ↓ GenT } }).
+    apply_fresh ty_let as TLlet.
+    - apply_fresh ty_new_intro as TLself; crush.
+    - crush.
+      match goal with
+      | [ |- ?G ⊢ ?t : ?T ] =>
+        assert (HR: open_typ_p (pvar TLlet) T = T) by crush;
+          rewrite <- HR;
+          clear HR
+      end.
+      apply ty_rec_elim.
+      rewrite <- Heqenv.
+      apply ty_var.
+      solve_bind.
+  }
+
+  apply_fresh ty_let as res.
+  - apply_fresh ty_let as e1app1; crush.
+    1: {
+      eapply ty_all_elim.
+      - assert (HR: p_sel (avar_f eq1) [pmatch] = (pvar eq1) • pmatch) by crush.
+        rewrite HR.
+        apply ty_new_elim.
+        apply ty_sub with (open_typ_p (pvar eq1) (({Ai 1 >: ⊥ <: ⊤} ∧ {Ai 2 >: ⊥ <: ⊤})
+                                                 ∧ {pmatch
+                                                      ⦂ ∀ ({GenT >: ⊥ <: ⊤}) (∀ (∀ ((pvar env ↓ GC Eq 0) ∧ {{super}})
+                                                                                   (super ↓ GenT)) (super ↓ GenT) ) })).
+        + apply ty_rec_elim.
+          apply ty_sub with (pvar env ↓ GN Eq).
+          * var_subtyp; crush.
+            repeat rewrite <- Heqenv.
+            eapply subtyp_trans; apply subtyp_and11.
+          * eapply subtyp_sel1.
+            match goal with
+            | [ |- context [ env ~ μ ?T ] ] =>
+              apply ty_sub with (open_typ_p (pvar env) T)
+            end.
+            -- apply ty_rec_elim. apply ty_var.
+               solve_bind.
+            -- crush.
+               eapply subtyp_trans; try apply subtyp_and11.
+        + crush.
+      - eapply ty_sub.
+        + apply ty_var. solve_bind.
+        + apply~ subtyp_typ.
+    }
+
+    crush.
+    apply_fresh ty_let as case1.
+    + match goal with
+      | [ |- context [ e1app1 ~ ∀ (?A) ?B ] ] =>
+        instantiate (1:=A)
+      end.
+      rewrite <- Heqenv.
+      apply_fresh ty_all_intro as eq_ev1.
+      crush.
+      apply_fresh ty_let as e2app1.
+      1: {
+        eapply ty_all_elim.
+        - assert (HR: p_sel (avar_f eq2) [pmatch] = (pvar eq2) • pmatch) by crush.
+          rewrite HR.
+          apply ty_new_elim.
+          apply ty_sub with (open_typ_p (pvar eq2) (({Ai 1 >: ⊥ <: ⊤} ∧ {Ai 2 >: ⊥ <: ⊤})
+                                                    ∧ {pmatch
+                                                         ⦂ ∀ ({GenT >: ⊥ <: ⊤}) (∀ (∀ ((pvar env ↓ GC Eq 0) ∧ {{super}})
+                                                                                      (super ↓ GenT)) (super ↓ GenT) ) })).
+          + apply ty_rec_elim.
+            apply ty_sub with (pvar env ↓ GN Eq).
+            * var_subtyp; crush.
+              repeat rewrite <- Heqenv.
+              eapply subtyp_trans; apply subtyp_and11.
+            * eapply subtyp_sel1.
+              match goal with
+              | [ |- context [ env ~ μ ?T ] ] =>
+                apply ty_sub with (open_typ_p (pvar env) T)
+              end.
+              -- apply ty_rec_elim. apply ty_var.
+                 solve_bind.
+              -- crush.
+                 eapply subtyp_trans; try apply subtyp_and11.
+          + crush.
+        - eapply ty_sub.
+          + apply ty_var. solve_bind.
+          + apply~ subtyp_typ.
+      }
+
+      crush.
+      apply_fresh ty_let as case2.
+      * match goal with
+        | [ |- context [ e2app1 ~ ∀ (?A) ?B ] ] =>
+          instantiate (1:=A)
+        end.
+        apply_fresh ty_all_intro as eq_ev2.
+        crush.
+        admit.
+      * crush.
+        match goal with
+        | [ |- ?G ⊢ ?e : ?T ] =>
+          assert (HR: T = open_typ_p (pvar case2) T) by crush;
+            rewrite HR;
+            clear HR
+        end.
+        eapply ty_all_elim;
+          apply ty_var; solve_bind.
+    + crush.
+      match goal with
+      | [ |- context [ e1app1 ~ ∀ (?A) ?B ] ] =>
+        instantiate (1:=B)
+      end.
+      match goal with
+      | [ |- ?G ⊢ ?e : ?T ] =>
+        assert (HR: T = open_typ_p (pvar case1) T) by crush;
+          rewrite HR;
+          clear HR
+      end.
+      eapply ty_all_elim;
+        apply ty_var; solve_bind.
+  - crush.
+    eapply ty_sub.
+    + apply ty_var; solve_bind.
+    + eapply subtyp_sel1.
+      rewrite <- Heqenv.
+      crush.
+Admitted.
